<?xml version="1.0" encoding="UTF-8"?>
<rdf:RDF xmlns:rdf="http://www.w3.org/1999/02/22-rdf-syntax-ns#"
         xmlns:owl="http://www.w3.org/2002/07/owl#"
         xmlns:skos="http://www.w3.org/2004/02/skos/core#"
         xmlns:rdfs="http://www.w3.org/2000/01/rdf-schema#"
         xmlns:at="http://publications.europa.eu/ontology/authority/"
         xmlns:dc="http://purl.org/dc/elements/1.1/"
         xmlns:atold="http://publications.europa.eu/resource/authority/"
         xml:base="http://publications.europa.eu/resource/authority/subdivision">
    <skos:ConceptScheme rdf:about="http://publications.europa.eu/resource/authority/subdivision"
                        at:table.id="subdivision"
                        at:table.version.number="20241211-0">
        <owl:versionInfo>20241211-0</owl:versionInfo>
        <skos:prefLabel xml:lang="en">Subdivision</skos:prefLabel>
        <rdfs:label xml:lang="en">Subdivision</rdfs:label>
        <at:prefLabel xml:lang="en">Subdivision</at:prefLabel>
        <skos:hasTopConcept rdf:resource="http://publications.europa.eu/resource/authority/subdivision/EXL"/>
        <skos:hasTopConcept rdf:resource="http://publications.europa.eu/resource/authority/subdivision/TIS"/>
        <skos:hasTopConcept rdf:resource="http://publications.europa.eu/resource/authority/subdivision/APP"/>
        <skos:hasTopConcept rdf:resource="http://publications.europa.eu/resource/authority/subdivision/LLG"/>
        <skos:hasTopConcept rdf:resource="http://publications.europa.eu/resource/authority/subdivision/COR"/>
        <skos:hasTopConcept rdf:resource="http://publications.europa.eu/resource/authority/subdivision/TXN"/>
        <skos:hasTopConcept rdf:resource="http://publications.europa.eu/resource/authority/subdivision/ENC"/>
        <skos:hasTopConcept rdf:resource="http://publications.europa.eu/resource/authority/subdivision/TOC"/>
        <skos:hasTopConcept rdf:resource="http://publications.europa.eu/resource/authority/subdivision/COL"/>
        <skos:hasTopConcept rdf:resource="http://publications.europa.eu/resource/authority/subdivision/OTH"/>
        <skos:hasTopConcept rdf:resource="http://publications.europa.eu/resource/authority/subdivision/ALN"/>
        <skos:hasTopConcept rdf:resource="http://publications.europa.eu/resource/authority/subdivision/SBS"/>
        <skos:hasTopConcept rdf:resource="http://publications.europa.eu/resource/authority/subdivision/ACT"/>
        <skos:hasTopConcept rdf:resource="http://publications.europa.eu/resource/authority/subdivision/UNP"/>
        <skos:hasTopConcept rdf:resource="http://publications.europa.eu/resource/authority/subdivision/CLS"/>
        <skos:hasTopConcept rdf:resource="http://publications.europa.eu/resource/authority/subdivision/CPT"/>
        <skos:hasTopConcept rdf:resource="http://publications.europa.eu/resource/authority/subdivision/TBG"/>
        <skos:hasTopConcept rdf:resource="http://publications.europa.eu/resource/authority/subdivision/NOT"/>
        <skos:hasTopConcept rdf:resource="http://publications.europa.eu/resource/authority/subdivision/PTA"/>
        <skos:hasTopConcept rdf:resource="http://publications.europa.eu/resource/authority/subdivision/WRP"/>
        <skos:hasTopConcept rdf:resource="http://publications.europa.eu/resource/authority/subdivision/DES"/>
        <skos:hasTopConcept rdf:resource="http://publications.europa.eu/resource/authority/subdivision/FTN"/>
        <skos:hasTopConcept rdf:resource="http://publications.europa.eu/resource/authority/subdivision/FNA"/>
        <skos:hasTopConcept rdf:resource="http://publications.europa.eu/resource/authority/subdivision/ART"/>
        <skos:hasTopConcept rdf:resource="http://publications.europa.eu/resource/authority/subdivision/CIT"/>
        <skos:hasTopConcept rdf:resource="http://publications.europa.eu/resource/authority/subdivision/ITM"/>
        <skos:hasTopConcept rdf:resource="http://publications.europa.eu/resource/authority/subdivision/LTR"/>
        <skos:hasTopConcept rdf:resource="http://publications.europa.eu/resource/authority/subdivision/IDT"/>
        <skos:hasTopConcept rdf:resource="http://publications.europa.eu/resource/authority/subdivision/PCD"/>
        <skos:hasTopConcept rdf:resource="http://publications.europa.eu/resource/authority/subdivision/DCL"/>
        <skos:hasTopConcept rdf:resource="http://publications.europa.eu/resource/authority/subdivision/ANX"/>
        <skos:hasTopConcept rdf:resource="http://publications.europa.eu/resource/authority/subdivision/PBL"/>
        <skos:hasTopConcept rdf:resource="http://publications.europa.eu/resource/authority/subdivision/SFR"/>
        <skos:hasTopConcept rdf:resource="http://publications.europa.eu/resource/authority/subdivision/SCT"/>
        <skos:hasTopConcept rdf:resource="http://publications.europa.eu/resource/authority/subdivision/FGR"/>
        <skos:hasTopConcept rdf:resource="http://publications.europa.eu/resource/authority/subdivision/LST"/>
        <skos:hasTopConcept rdf:resource="http://publications.europa.eu/resource/authority/subdivision/SUB"/>
        <skos:hasTopConcept rdf:resource="http://publications.europa.eu/resource/authority/subdivision/SNT"/>
        <skos:hasTopConcept rdf:resource="http://publications.europa.eu/resource/authority/subdivision/RCT"/>
        <skos:hasTopConcept rdf:resource="http://publications.europa.eu/resource/authority/subdivision/TAB"/>
        <skos:hasTopConcept rdf:resource="http://publications.europa.eu/resource/authority/subdivision/ROW"/>
        <skos:hasTopConcept rdf:resource="http://publications.europa.eu/resource/authority/subdivision/INP"/>
        <skos:hasTopConcept rdf:resource="http://publications.europa.eu/resource/authority/subdivision/CGR"/>
        <skos:hasTopConcept rdf:resource="http://publications.europa.eu/resource/authority/subdivision/IMG"/>
        <skos:hasTopConcept rdf:resource="http://publications.europa.eu/resource/authority/subdivision/PNT"/>
        <skos:hasTopConcept rdf:resource="http://publications.europa.eu/resource/authority/subdivision/AGR"/>
        <skos:hasTopConcept rdf:resource="http://publications.europa.eu/resource/authority/subdivision/FNP"/>
        <skos:hasTopConcept rdf:resource="http://publications.europa.eu/resource/authority/subdivision/PRO"/>
        <skos:hasTopConcept rdf:resource="http://publications.europa.eu/resource/authority/subdivision/MNT"/>
        <skos:hasTopConcept rdf:resource="http://publications.europa.eu/resource/authority/subdivision/CNV"/>
        <skos:hasTopConcept rdf:resource="http://publications.europa.eu/resource/authority/subdivision/TIT"/>
        <skos:hasTopConcept rdf:resource="http://publications.europa.eu/resource/authority/subdivision/LGD"/>
        <skos:hasTopConcept rdf:resource="http://publications.europa.eu/resource/authority/subdivision/RUL"/>
        <skos:hasTopConcept rdf:resource="http://publications.europa.eu/resource/authority/subdivision/PAG"/>
        <skos:hasTopConcept rdf:resource="http://publications.europa.eu/resource/authority/subdivision/PRT"/>
        <skos:hasTopConcept rdf:resource="http://publications.europa.eu/resource/authority/subdivision/TXO"/>
        <skos:hasTopConcept rdf:resource="http://publications.europa.eu/resource/authority/subdivision/END"/>
        <skos:hasTopConcept rdf:resource="http://publications.europa.eu/resource/authority/subdivision/PTI"/>
        <skos:hasTopConcept rdf:resource="http://publications.europa.eu/resource/authority/subdivision/PAR"/>
        <skos:hasTopConcept rdf:resource="http://publications.europa.eu/resource/authority/subdivision/OP_DATPRO"/>
    </skos:ConceptScheme>
    <skos:Concept rdf:about="http://publications.europa.eu/resource/authority/subdivision/EXL"
                  at:deprecated="false">
        <skos:prefLabel xml:lang="sv">skriftväxling</skos:prefLabel>
        <skos:prefLabel xml:lang="en">exchange of letters</skos:prefLabel>
        <skos:definition xml:lang="en">This element indicates an exchange of letters, a specific part of a document,
            e.g. in a treaty.
        </skos:definition>
        <skos:inScheme rdf:resource="http://publications.europa.eu/resource/authority/subdivision"/>
        <skos:topConceptOf rdf:resource="http://publications.europa.eu/resource/authority/subdivision"/>
        <dc:identifier>EXL</dc:identifier>
        <atold:op-code>EXL</atold:op-code>
        <at:op-code>EXL</at:op-code>
        <at:start.use>1952-12-30</at:start.use>
        <at:authority-code>EXL</at:authority-code>
    </skos:Concept>
    <skos:Concept rdf:about="http://publications.europa.eu/resource/authority/subdivision/TIS"
                  at:deprecated="false">
        <skos:prefLabel xml:lang="sv">avdelning (del)</skos:prefLabel>
        <skos:prefLabel xml:lang="en">title (subdivision)</skos:prefLabel>
        <skos:definition xml:lang="en">higher subdivision of an act positioned between part and chapter used to
            introduce a group of articles in the enacting terms
        </skos:definition>
        <skos:inScheme rdf:resource="http://publications.europa.eu/resource/authority/subdivision"/>
        <skos:topConceptOf rdf:resource="http://publications.europa.eu/resource/authority/subdivision"/>
        <dc:identifier>TIS</dc:identifier>
        <atold:op-code>TIS</atold:op-code>
        <at:op-code>TIS</at:op-code>
        <at:start.use>1952-12-30</at:start.use>
        <at:authority-code>TIS</at:authority-code>
        <skos:scopeNote xml:lang="en">Indicates in long and highly structured texts the grouping of higher subdivisions
            (JPG 15.4, p. 28).
        </skos:scopeNote>
        <skos:scopeNote xml:lang="en">Titles have distinctive signs of type uppercase Roman numbers I, II, III etc.
        </skos:scopeNote>
        <skos:notation rdf:datatype="http://publications.europa.eu/ontology/euvoc#FORMEX">TT</skos:notation>
        <at:op-mapped-code>
            <at:MappedCode>
                <dc:source>FORMEX</dc:source>
                <at:legacy-code>TT</at:legacy-code>
            </at:MappedCode>
        </at:op-mapped-code>
    </skos:Concept>
    <skos:Concept rdf:about="http://publications.europa.eu/resource/authority/subdivision/APP"
                  at:deprecated="false">
        <skos:prefLabel xml:lang="sv">tillägg</skos:prefLabel>
        <skos:prefLabel xml:lang="en">appendix</skos:prefLabel>
        <skos:definition xml:lang="en">An appendix is a distinct supplementary part of an act which generally contains
            explanatory or statistical information, and which frequently take the form of a list or table.
        </skos:definition>
        <skos:inScheme rdf:resource="http://publications.europa.eu/resource/authority/subdivision"/>
        <skos:topConceptOf rdf:resource="http://publications.europa.eu/resource/authority/subdivision"/>
        <dc:identifier>APP</dc:identifier>
        <atold:op-code>APP</atold:op-code>
        <at:op-code>APP</at:op-code>
        <at:start.use>2015-03-18</at:start.use>
        <at:authority-code>APP</at:authority-code>
        <skos:notation rdf:datatype="http://publications.europa.eu/ontology/euvoc#FORMEX">AP</skos:notation>
        <at:op-mapped-code>
            <at:MappedCode>
                <dc:source>FORMEX</dc:source>
                <at:legacy-code>AP</at:legacy-code>
            </at:MappedCode>
        </at:op-mapped-code>
    </skos:Concept>
    <skos:Concept rdf:about="http://publications.europa.eu/resource/authority/subdivision/LLG"
                  at:deprecated="false">
        <skos:prefLabel xml:lang="sv">rad i förklaring</skos:prefLabel>
        <skos:prefLabel xml:lang="en">line of legend</skos:prefLabel>
        <skos:definition xml:lang="en">In a legend, a line of legend is a description of an individual element.
        </skos:definition>
        <skos:inScheme rdf:resource="http://publications.europa.eu/resource/authority/subdivision"/>
        <skos:topConceptOf rdf:resource="http://publications.europa.eu/resource/authority/subdivision"/>
        <dc:identifier>LLG</dc:identifier>
        <atold:op-code>LLG</atold:op-code>
        <at:op-code>LLG</at:op-code>
        <at:start.use>1952-12-30</at:start.use>
        <at:authority-code>LLG</at:authority-code>
    </skos:Concept>
    <skos:Concept rdf:about="http://publications.europa.eu/resource/authority/subdivision/COR"
                  at:deprecated="false">
        <skos:prefLabel xml:lang="en">correction</skos:prefLabel>
        <skos:prefLabel xml:lang="sv">rättelse</skos:prefLabel>
        <skos:definition xml:lang="en">This element is specific to the corrigendum type of document. It is used to mark
            up the details about the correction/modification asked for a legal document after its publication.
        </skos:definition>
        <skos:inScheme rdf:resource="http://publications.europa.eu/resource/authority/subdivision"/>
        <skos:topConceptOf rdf:resource="http://publications.europa.eu/resource/authority/subdivision"/>
        <dc:identifier>COR</dc:identifier>
        <atold:op-code>COR</atold:op-code>
        <at:op-code>COR</at:op-code>
        <at:start.use>2004-05-01</at:start.use>
        <at:authority-code>COR</at:authority-code>
    </skos:Concept>
    <skos:Concept rdf:about="http://publications.europa.eu/resource/authority/subdivision/TXN"
                  at:deprecated="false">
        <skos:prefLabel xml:lang="en">new text</skos:prefLabel>
        <skos:prefLabel xml:lang="sv">ny text</skos:prefLabel>
        <skos:definition xml:lang="en">This element is specific to the corrigendum type of document. It is a subdivision
            of the correction and is used to mark up the new text that should replace the old one in a legal document.
        </skos:definition>
        <skos:inScheme rdf:resource="http://publications.europa.eu/resource/authority/subdivision"/>
        <skos:topConceptOf rdf:resource="http://publications.europa.eu/resource/authority/subdivision"/>
        <dc:identifier>TXN</dc:identifier>
        <atold:op-code>TXN</atold:op-code>
        <at:op-code>TXN</at:op-code>
        <at:start.use>2004-05-01</at:start.use>
        <at:authority-code>TXN</at:authority-code>
    </skos:Concept>
    <skos:Concept rdf:about="http://publications.europa.eu/resource/authority/subdivision/ENC"
                  at:deprecated="false">
        <skos:prefLabel xml:lang="sv">artikeldel</skos:prefLabel>
        <skos:prefLabel xml:lang="en">enacting terms</skos:prefLabel>
        <skos:definition xml:lang="en">operative part of a legal document which follows the preamble</skos:definition>
        <skos:altLabel xml:lang="sv">normativ del</skos:altLabel>
        <skos:inScheme rdf:resource="http://publications.europa.eu/resource/authority/subdivision"/>
        <skos:topConceptOf rdf:resource="http://publications.europa.eu/resource/authority/subdivision"/>
        <dc:identifier>ENC</dc:identifier>
        <atold:op-code>ENC</atold:op-code>
        <at:op-code>ENC</at:op-code>
        <at:start.use>1952-12-30</at:start.use>
        <at:authority-code>ENC</at:authority-code>
        <skos:scopeNote xml:lang="en">Comprising for example the legal definitions.</skos:scopeNote>
        <skos:notation rdf:datatype="http://publications.europa.eu/ontology/euvoc#FORMEX">DI</skos:notation>
        <at:op-mapped-code>
            <at:MappedCode>
                <dc:source>FORMEX</dc:source>
                <at:legacy-code>DI</at:legacy-code>
            </at:MappedCode>
        </at:op-mapped-code>
    </skos:Concept>
    <skos:Concept rdf:about="http://publications.europa.eu/resource/authority/subdivision/TOC"
                  at:deprecated="false">
        <skos:prefLabel xml:lang="sv">innehållsförteckning</skos:prefLabel>
        <skos:prefLabel xml:lang="en">table of contents</skos:prefLabel>
        <skos:definition xml:lang="en">list of headings and subjects of a document, presented in the order in which they
            appear
        </skos:definition>
        <skos:inScheme rdf:resource="http://publications.europa.eu/resource/authority/subdivision"/>
        <skos:topConceptOf rdf:resource="http://publications.europa.eu/resource/authority/subdivision"/>
        <dc:identifier>TOC</dc:identifier>
        <atold:op-code>TOC</atold:op-code>
        <at:op-code>TOC</at:op-code>
        <at:start.use>1952-12-30</at:start.use>
        <at:authority-code>TOC</at:authority-code>
        <skos:notation rdf:datatype="http://publications.europa.eu/ontology/euvoc#FORMEX">SU</skos:notation>
        <at:op-mapped-code>
            <at:MappedCode>
                <dc:source>FORMEX</dc:source>
                <at:legacy-code>SU</at:legacy-code>
            </at:MappedCode>
        </at:op-mapped-code>
    </skos:Concept>
    <skos:Concept rdf:about="http://publications.europa.eu/resource/authority/subdivision/COL"
                  at:deprecated="false">
        <skos:prefLabel xml:lang="sv">tabellkolumn</skos:prefLabel>
        <skos:prefLabel xml:lang="en">table column</skos:prefLabel>
        <skos:definition xml:lang="en">vertical arrangement of data in a table</skos:definition>
        <skos:inScheme rdf:resource="http://publications.europa.eu/resource/authority/subdivision"/>
        <skos:topConceptOf rdf:resource="http://publications.europa.eu/resource/authority/subdivision"/>
        <dc:identifier>COL</dc:identifier>
        <atold:op-code>COL</atold:op-code>
        <at:op-code>COL</at:op-code>
        <at:start.use>1952-12-30</at:start.use>
        <at:authority-code>COL</at:authority-code>
    </skos:Concept>
    <skos:Concept rdf:about="http://publications.europa.eu/resource/authority/subdivision/OTH"
                  at:deprecated="false">
        <skos:prefLabel xml:lang="sv">andra</skos:prefLabel>
        <skos:prefLabel xml:lang="en">other</skos:prefLabel>
        <skos:definition xml:lang="en">This element indicates any non specified subdivision.</skos:definition>
        <skos:inScheme rdf:resource="http://publications.europa.eu/resource/authority/subdivision"/>
        <skos:topConceptOf rdf:resource="http://publications.europa.eu/resource/authority/subdivision"/>
        <dc:identifier>OTH</dc:identifier>
        <atold:op-code>OTH</atold:op-code>
        <at:op-code>OTH</at:op-code>
        <at:start.use>1952-07-24</at:start.use>
        <at:authority-code>OTH</at:authority-code>
    </skos:Concept>
    <skos:Concept rdf:about="http://publications.europa.eu/resource/authority/subdivision/ALN"
                  at:deprecated="false">
        <skos:prefLabel xml:lang="en">unnumbered paragraph</skos:prefLabel>
        <skos:prefLabel xml:lang="sv">stycke</skos:prefLabel>
        <skos:definition xml:lang="en">sole element or a non-independent element of an article (JPG 15.4, table) or
            exceptionally an element of an annex
        </skos:definition>
        <skos:altLabel xml:lang="en">sub-paragraph</skos:altLabel>
        <skos:inScheme rdf:resource="http://publications.europa.eu/resource/authority/subdivision"/>
        <skos:topConceptOf rdf:resource="http://publications.europa.eu/resource/authority/subdivision"/>
        <dc:identifier>ALN</dc:identifier>
        <atold:op-code>ALN</atold:op-code>
        <at:op-code>ALN</at:op-code>
        <at:start.use>2015-03-18</at:start.use>
        <at:authority-code>ALN</at:authority-code>
        <skos:scopeNote xml:lang="en">Subdivision of an article which does not have a distinctive sign (number, letter
            or dash).
        </skos:scopeNote>
        <skos:notation rdf:datatype="http://publications.europa.eu/ontology/euvoc#CJ">L</skos:notation>
        <skos:notation rdf:datatype="http://publications.europa.eu/ontology/euvoc#FORMEX">AL</skos:notation>
        <at:op-mapped-code>
            <at:MappedCode>
                <dc:source>CJ</dc:source>
                <at:legacy-code>L</at:legacy-code>
            </at:MappedCode>
        </at:op-mapped-code>
        <at:op-mapped-code>
            <at:MappedCode>
                <dc:source>FORMEX</dc:source>
                <at:legacy-code>AL</at:legacy-code>
            </at:MappedCode>
        </at:op-mapped-code>
    </skos:Concept>
    <skos:Concept rdf:about="http://publications.europa.eu/resource/authority/subdivision/SBS"
                  at:deprecated="false">
        <skos:prefLabel xml:lang="en">subsection</skos:prefLabel>
        <skos:prefLabel xml:lang="sv">underavsnitt</skos:prefLabel>
        <skos:definition xml:lang="en">This element indicates a subclause in the regular structure of a legal document
            below the level of a section. Example: Council Regulation (EC) No 491/2009 of 25 May 2009.
        </skos:definition>
        <skos:inScheme rdf:resource="http://publications.europa.eu/resource/authority/subdivision"/>
        <skos:topConceptOf rdf:resource="http://publications.europa.eu/resource/authority/subdivision"/>
        <dc:identifier>SBS</dc:identifier>
        <atold:op-code>SBS</atold:op-code>
        <at:op-code>SBS</at:op-code>
        <at:start.use>1952-12-30</at:start.use>
        <at:authority-code>SBS</at:authority-code>
        <skos:notation rdf:datatype="http://publications.europa.eu/ontology/euvoc#FORMEX">SD</skos:notation>
        <at:op-mapped-code>
            <at:MappedCode>
                <dc:source>FORMEX</dc:source>
                <at:legacy-code>SD</at:legacy-code>
            </at:MappedCode>
        </at:op-mapped-code>
    </skos:Concept>
    <skos:Concept rdf:about="http://publications.europa.eu/resource/authority/subdivision/ACT"
                  at:deprecated="false">
        <skos:prefLabel xml:lang="en">act</skos:prefLabel>
        <skos:prefLabel xml:lang="sv">akt</skos:prefLabel>
        <skos:definition xml:lang="en">This element indicates a differentiated legal act, e.g. in the context of an
            accession treaty.
        </skos:definition>
        <skos:inScheme rdf:resource="http://publications.europa.eu/resource/authority/subdivision"/>
        <skos:topConceptOf rdf:resource="http://publications.europa.eu/resource/authority/subdivision"/>
        <dc:identifier>ACT</dc:identifier>
        <atold:op-code>ACT</atold:op-code>
        <at:op-code>ACT</at:op-code>
        <at:start.use>1952-12-30</at:start.use>
        <at:authority-code>ACT</at:authority-code>
    </skos:Concept>
    <skos:Concept rdf:about="http://publications.europa.eu/resource/authority/subdivision/UNP"
                  at:deprecated="false">
        <skos:prefLabel xml:lang="en">unnumbered paragraph</skos:prefLabel>
        <skos:prefLabel xml:lang="sv">stycke</skos:prefLabel>
        <skos:definition xml:lang="en">unnumbered subdivision of an article or, exceptionally an element of an annex
        </skos:definition>
        <skos:inScheme rdf:resource="http://publications.europa.eu/resource/authority/subdivision"/>
        <skos:topConceptOf rdf:resource="http://publications.europa.eu/resource/authority/subdivision"/>
        <dc:identifier>UNP</dc:identifier>
        <atold:op-code>UNP</atold:op-code>
        <at:op-code>UNP</at:op-code>
        <at:start.use>1952-12-30</at:start.use>
        <at:authority-code>UNP</at:authority-code>
        <skos:scopeNote xml:lang="en">If an article is not subdivided, i.e. has only one paragraph, it is an unnumbered
            paragraph.
        </skos:scopeNote>
    </skos:Concept>
    <skos:Concept rdf:about="http://publications.europa.eu/resource/authority/subdivision/CLS"
                  at:deprecated="false">
        <skos:prefLabel xml:lang="en">clause</skos:prefLabel>
        <skos:prefLabel xml:lang="sv">klausul</skos:prefLabel>
        <skos:definition xml:lang="en">A clause is a distinct provision at the end of an agreement, a treaty or another
            act.
        </skos:definition>
        <skos:inScheme rdf:resource="http://publications.europa.eu/resource/authority/subdivision"/>
        <skos:topConceptOf rdf:resource="http://publications.europa.eu/resource/authority/subdivision"/>
        <dc:identifier>CLS</dc:identifier>
        <atold:op-code>CLS</atold:op-code>
        <at:op-code>CLS</at:op-code>
        <at:start.use>2015-03-18</at:start.use>
        <at:authority-code>CLS</at:authority-code>
        <skos:notation rdf:datatype="http://publications.europa.eu/ontology/euvoc#CJ">CL</skos:notation>
        <at:op-mapped-code>
            <at:MappedCode>
                <dc:source>CJ</dc:source>
                <at:legacy-code>CL</at:legacy-code>
            </at:MappedCode>
        </at:op-mapped-code>
    </skos:Concept>
    <skos:Concept rdf:about="http://publications.europa.eu/resource/authority/subdivision/CPT"
                  at:deprecated="false">
        <skos:prefLabel xml:lang="sv">kapitel</skos:prefLabel>
        <skos:prefLabel xml:lang="en">chapter</skos:prefLabel>
        <skos:definition xml:lang="en">higher subdivision within a legal act used to introduce a group of articles in
            the enacting terms
        </skos:definition>
        <skos:inScheme rdf:resource="http://publications.europa.eu/resource/authority/subdivision"/>
        <skos:topConceptOf rdf:resource="http://publications.europa.eu/resource/authority/subdivision"/>
        <dc:identifier>CPT</dc:identifier>
        <atold:op-code>CPT</atold:op-code>
        <at:op-code>CPT</at:op-code>
        <at:start.use>2015-03-18</at:start.use>
        <at:authority-code>CPT</at:authority-code>
        <skos:scopeNote xml:lang="en">In the hierarchy of subdivisions, chapter is between title and section.
        </skos:scopeNote>
        <skos:scopeNote xml:lang="en">Chapters have distinctive signs of type Arab numerals 1, 2, 3 etc. or uppercase
            Roman numbers I, II, III etc.
        </skos:scopeNote>
        <skos:notation rdf:datatype="http://publications.europa.eu/ontology/euvoc#FORMEX">CH</skos:notation>
        <skos:notation rdf:datatype="http://publications.europa.eu/ontology/euvoc#CJ">CH</skos:notation>
        <at:op-mapped-code>
            <at:MappedCode>
                <dc:source>CJ</dc:source>
                <at:legacy-code>CH</at:legacy-code>
            </at:MappedCode>
        </at:op-mapped-code>
        <at:op-mapped-code>
            <at:MappedCode>
                <dc:source>FORMEX</dc:source>
                <at:legacy-code>CH</at:legacy-code>
            </at:MappedCode>
        </at:op-mapped-code>
    </skos:Concept>
    <skos:Concept rdf:about="http://publications.europa.eu/resource/authority/subdivision/TBG"
                  at:deprecated="false">
        <skos:prefLabel xml:lang="en">group of tables</skos:prefLabel>
        <skos:prefLabel xml:lang="sv">grupp av tabeller</skos:prefLabel>
        <skos:definition xml:lang="en">This element is used to group tables together that share a common title or a
            common note.
        </skos:definition>
        <skos:inScheme rdf:resource="http://publications.europa.eu/resource/authority/subdivision"/>
        <skos:topConceptOf rdf:resource="http://publications.europa.eu/resource/authority/subdivision"/>
        <dc:identifier>TBG</dc:identifier>
        <atold:op-code>TBG</atold:op-code>
        <at:op-code>TBG</at:op-code>
        <at:start.use>2004-05-01</at:start.use>
        <at:authority-code>TBG</at:authority-code>
    </skos:Concept>
    <skos:Concept rdf:about="http://publications.europa.eu/resource/authority/subdivision/NOT"
                  at:deprecated="false">
        <skos:prefLabel xml:lang="sv">anmärkning</skos:prefLabel>
        <skos:prefLabel xml:lang="en">note</skos:prefLabel>
        <skos:definition xml:lang="en">specific additional explanatory part of a legal document</skos:definition>
        <skos:inScheme rdf:resource="http://publications.europa.eu/resource/authority/subdivision"/>
        <skos:topConceptOf rdf:resource="http://publications.europa.eu/resource/authority/subdivision"/>
        <dc:identifier>NOT</dc:identifier>
        <atold:op-code>NOT</atold:op-code>
        <at:op-code>NOT</at:op-code>
        <at:start.use>1952-12-30</at:start.use>
        <at:authority-code>NOT</at:authority-code>
        <skos:example xml:lang="en">Commission Directive (EU) 2015/1787 of 6 October 2015</skos:example>
    </skos:Concept>
    <skos:Concept rdf:about="http://publications.europa.eu/resource/authority/subdivision/PTA"
                  at:deprecated="false">
        <skos:prefLabel xml:lang="en">point</skos:prefLabel>
        <skos:prefLabel xml:lang="sv">led</skos:prefLabel>
        <skos:definition xml:lang="en">structure component of a legal article that has a distinctive sign of the type
            lowercase letters: (a), (b), (c) etc.
        </skos:definition>
        <skos:inScheme rdf:resource="http://publications.europa.eu/resource/authority/subdivision"/>
        <skos:topConceptOf rdf:resource="http://publications.europa.eu/resource/authority/subdivision"/>
        <dc:identifier>PTA</dc:identifier>
        <atold:op-code>PTA</atold:op-code>
        <at:op-code>PTA</at:op-code>
        <at:start.use>1952-12-30</at:start.use>
        <at:authority-code>PTA</at:authority-code>
    </skos:Concept>
    <skos:Concept rdf:about="http://publications.europa.eu/resource/authority/subdivision/WRP"
                  at:deprecated="false">
        <skos:prefLabel xml:lang="en">closing part</skos:prefLabel>
        <skos:prefLabel xml:lang="sv">slutdel</skos:prefLabel>
        <skos:definition xml:lang="en">part that follows the enumeration in a sentence that includes an enumeration of
            points or indents
        </skos:definition>
        <skos:inScheme rdf:resource="http://publications.europa.eu/resource/authority/subdivision"/>
        <skos:topConceptOf rdf:resource="http://publications.europa.eu/resource/authority/subdivision"/>
        <dc:identifier>WRP</dc:identifier>
        <atold:op-code>WRP</atold:op-code>
        <at:op-code>WRP</at:op-code>
        <at:start.use>1952-12-30</at:start.use>
        <at:authority-code>WRP</at:authority-code>
    </skos:Concept>
    <skos:Concept rdf:about="http://publications.europa.eu/resource/authority/subdivision/DES"
                  at:deprecated="false">
        <skos:prefLabel xml:lang="sv">beskrivning</skos:prefLabel>
        <skos:prefLabel xml:lang="en">description</skos:prefLabel>
        <skos:definition xml:lang="en">This element is specific to the corrigendum type of document. It is a subdivision
            of the correction and is used to mark up the details (subject, location) where the modification should be
            implemented in a legal document.
        </skos:definition>
        <skos:inScheme rdf:resource="http://publications.europa.eu/resource/authority/subdivision"/>
        <skos:topConceptOf rdf:resource="http://publications.europa.eu/resource/authority/subdivision"/>
        <dc:identifier>DES</dc:identifier>
        <atold:op-code>DES</atold:op-code>
        <at:op-code>DES</at:op-code>
        <at:start.use>2004-05-01</at:start.use>
        <at:authority-code>DES</at:authority-code>
    </skos:Concept>
    <skos:Concept rdf:about="http://publications.europa.eu/resource/authority/subdivision/FTN"
                  at:deprecated="false">
        <skos:prefLabel xml:lang="sv">fotnot</skos:prefLabel>
        <skos:prefLabel xml:lang="en">footnote</skos:prefLabel>
        <skos:definition xml:lang="en">reference included in a legal document which is specified at the bottom of the
            same page
        </skos:definition>
        <skos:inScheme rdf:resource="http://publications.europa.eu/resource/authority/subdivision"/>
        <skos:topConceptOf rdf:resource="http://publications.europa.eu/resource/authority/subdivision"/>
        <dc:identifier>FTN</dc:identifier>
        <atold:op-code>FTN</atold:op-code>
        <at:op-code>FTN</at:op-code>
        <at:start.use>1952-12-30</at:start.use>
        <at:authority-code>FTN</at:authority-code>
        <skos:notation rdf:datatype="http://publications.europa.eu/ontology/euvoc#FORMEX">FN</skos:notation>
        <at:op-mapped-code>
            <at:MappedCode>
                <dc:source>FORMEX</dc:source>
                <at:legacy-code>FN</at:legacy-code>
            </at:MappedCode>
        </at:op-mapped-code>
    </skos:Concept>
    <skos:Concept rdf:about="http://publications.europa.eu/resource/authority/subdivision/FNA"
                  at:deprecated="false">
        <skos:prefLabel xml:lang="en">final act</skos:prefLabel>
        <skos:prefLabel xml:lang="sv">slutakt</skos:prefLabel>
        <skos:definition xml:lang="en">This element indicates a final act, a specific part of a document, in general in
            international agreements.
        </skos:definition>
        <skos:inScheme rdf:resource="http://publications.europa.eu/resource/authority/subdivision"/>
        <skos:topConceptOf rdf:resource="http://publications.europa.eu/resource/authority/subdivision"/>
        <dc:identifier>FNA</dc:identifier>
        <atold:op-code>FNA</atold:op-code>
        <at:op-code>FNA</at:op-code>
        <at:start.use>1952-12-30</at:start.use>
        <at:authority-code>FNA</at:authority-code>
        <skos:notation rdf:datatype="http://publications.europa.eu/ontology/euvoc#FORMEX">FA</skos:notation>
        <at:op-mapped-code>
            <at:MappedCode>
                <dc:source>FORMEX</dc:source>
                <at:legacy-code>FA</at:legacy-code>
            </at:MappedCode>
        </at:op-mapped-code>
    </skos:Concept>
    <skos:Concept rdf:about="http://publications.europa.eu/resource/authority/subdivision/ART"
                  at:deprecated="false">
        <skos:prefLabel xml:lang="en">article</skos:prefLabel>
        <skos:prefLabel xml:lang="sv">artikel</skos:prefLabel>
        <skos:definition xml:lang="en">basic component of the enacting terms of a legal act</skos:definition>
        <skos:inScheme rdf:resource="http://publications.europa.eu/resource/authority/subdivision"/>
        <skos:topConceptOf rdf:resource="http://publications.europa.eu/resource/authority/subdivision"/>
        <dc:identifier>ART</dc:identifier>
        <atold:op-code>ART</atold:op-code>
        <at:op-code>ART</at:op-code>
        <at:start.use>2015-03-18</at:start.use>
        <at:authority-code>ART</at:authority-code>
        <skos:scopeNote xml:lang="en">Distinguishable by the standardised title, which consists of the expression
            ‘Article’ followed by a sequential number or preceded by ‘sole’.
        </skos:scopeNote>
        <skos:notation rdf:datatype="http://publications.europa.eu/ontology/euvoc#CJ">A</skos:notation>
        <skos:notation rdf:datatype="http://publications.europa.eu/ontology/euvoc#FORMEX">AR</skos:notation>
        <at:op-mapped-code>
            <at:MappedCode>
                <dc:source>FORMEX</dc:source>
                <at:legacy-code>AR</at:legacy-code>
            </at:MappedCode>
        </at:op-mapped-code>
        <at:op-mapped-code>
            <at:MappedCode>
                <dc:source>CJ</dc:source>
                <at:legacy-code>A</at:legacy-code>
            </at:MappedCode>
        </at:op-mapped-code>
    </skos:Concept>
    <skos:Concept rdf:about="http://publications.europa.eu/resource/authority/subdivision/CIT"
                  at:deprecated="false">
        <skos:prefLabel xml:lang="sv">beaktandeled</skos:prefLabel>
        <skos:prefLabel xml:lang="en">citation</skos:prefLabel>
        <skos:definition xml:lang="en">legal basis for an act or a preparatory act and in the case of a legislative act
            also the procedure followed and the transmission of a draft legislative act to national parliaments
        </skos:definition>
        <skos:inScheme rdf:resource="http://publications.europa.eu/resource/authority/subdivision"/>
        <skos:topConceptOf rdf:resource="http://publications.europa.eu/resource/authority/subdivision"/>
        <dc:identifier>CIT</dc:identifier>
        <atold:op-code>CIT</atold:op-code>
        <at:op-code>CIT</at:op-code>
        <at:start.use>2015-03-18</at:start.use>
        <at:authority-code>CIT</at:authority-code>
        <skos:scopeNote xml:lang="en">In the hierarchy, citations are elements of the preamble.</skos:scopeNote>
        <skos:notation rdf:datatype="http://publications.europa.eu/ontology/euvoc#FORMEX">VI</skos:notation>
        <at:op-mapped-code>
            <at:MappedCode>
                <dc:source>FORMEX</dc:source>
                <at:legacy-code>VI</at:legacy-code>
            </at:MappedCode>
        </at:op-mapped-code>
    </skos:Concept>
    <skos:Concept rdf:about="http://publications.europa.eu/resource/authority/subdivision/ITM"
                  at:deprecated="false">
        <skos:prefLabel xml:lang="en">item</skos:prefLabel>
        <skos:prefLabel xml:lang="sv">punkt</skos:prefLabel>
        <skos:definition xml:lang="en">subdivision of a bigger text, presented in the form of a list of interventions
        </skos:definition>
        <skos:inScheme rdf:resource="http://publications.europa.eu/resource/authority/subdivision"/>
        <skos:topConceptOf rdf:resource="http://publications.europa.eu/resource/authority/subdivision"/>
        <dc:identifier>ITM</dc:identifier>
        <atold:op-code>ITM</atold:op-code>
        <at:op-code>ITM</at:op-code>
        <at:start.use>1979-07-01</at:start.use>
        <at:authority-code>ITM</at:authority-code>
    </skos:Concept>
    <skos:Concept rdf:about="http://publications.europa.eu/resource/authority/subdivision/LTR"
                  at:deprecated="false">
        <skos:prefLabel xml:lang="sv">skrivelse</skos:prefLabel>
        <skos:prefLabel xml:lang="en">letter</skos:prefLabel>
        <skos:definition xml:lang="en">This element indicates a letter integrated into a document, in general in
            international agreements.
        </skos:definition>
        <skos:inScheme rdf:resource="http://publications.europa.eu/resource/authority/subdivision"/>
        <skos:topConceptOf rdf:resource="http://publications.europa.eu/resource/authority/subdivision"/>
        <dc:identifier>LTR</dc:identifier>
        <atold:op-code>LTR</atold:op-code>
        <at:op-code>LTR</at:op-code>
        <at:start.use>1952-12-30</at:start.use>
        <at:authority-code>LTR</at:authority-code>
        <skos:notation rdf:datatype="http://publications.europa.eu/ontology/euvoc#FORMEX">LT</skos:notation>
        <at:op-mapped-code>
            <at:MappedCode>
                <dc:source>FORMEX</dc:source>
                <at:legacy-code>LT</at:legacy-code>
            </at:MappedCode>
        </at:op-mapped-code>
    </skos:Concept>
    <skos:Concept rdf:about="http://publications.europa.eu/resource/authority/subdivision/IDT"
                  at:deprecated="false">
        <skos:prefLabel xml:lang="en">indent</skos:prefLabel>
        <skos:prefLabel xml:lang="sv">strecksats</skos:prefLabel>
        <skos:definition xml:lang="en">element of an enumeration preceded by a dash</skos:definition>
        <skos:inScheme rdf:resource="http://publications.europa.eu/resource/authority/subdivision"/>
        <skos:topConceptOf rdf:resource="http://publications.europa.eu/resource/authority/subdivision"/>
        <dc:identifier>IDT</dc:identifier>
        <atold:op-code>IDT</atold:op-code>
        <at:op-code>IDT</at:op-code>
        <at:start.use>2015-03-18</at:start.use>
        <at:authority-code>IDT</at:authority-code>
        <skos:scopeNote xml:lang="en">As indents have no figure nor other sign of identification, ordinal numbers
            written by letters are used to refer to them: first indent, second indent, third indent etc.
        </skos:scopeNote>
        <skos:notation rdf:datatype="http://publications.europa.eu/ontology/euvoc#FORMEX">DA</skos:notation>
        <skos:notation rdf:datatype="http://publications.europa.eu/ontology/euvoc#CJ">T</skos:notation>
        <at:op-mapped-code>
            <at:MappedCode>
                <dc:source>FORMEX</dc:source>
                <at:legacy-code>DA</at:legacy-code>
            </at:MappedCode>
        </at:op-mapped-code>
        <at:op-mapped-code>
            <at:MappedCode>
                <dc:source>CJ</dc:source>
                <at:legacy-code>T</at:legacy-code>
            </at:MappedCode>
        </at:op-mapped-code>
    </skos:Concept>
    <skos:Concept rdf:about="http://publications.europa.eu/resource/authority/subdivision/PCD"
                  at:deprecated="false">
        <skos:prefLabel xml:lang="en">procedure</skos:prefLabel>
        <skos:prefLabel xml:lang="sv">förfarande</skos:prefLabel>
        <skos:definition xml:lang="en">This element indicates a procedure, a specific part of a document, e.g. in a
            treaty.
        </skos:definition>
        <skos:inScheme rdf:resource="http://publications.europa.eu/resource/authority/subdivision"/>
        <skos:topConceptOf rdf:resource="http://publications.europa.eu/resource/authority/subdivision"/>
        <dc:identifier>PCD</dc:identifier>
        <atold:op-code>PCD</atold:op-code>
        <at:op-code>PCD</at:op-code>
        <at:start.use>1952-12-30</at:start.use>
        <at:authority-code>PCD</at:authority-code>
    </skos:Concept>
    <skos:Concept rdf:about="http://publications.europa.eu/resource/authority/subdivision/DCL"
                  at:deprecated="false">
        <skos:prefLabel xml:lang="en">declaration</skos:prefLabel>
        <skos:prefLabel xml:lang="sv">förklaring</skos:prefLabel>
        <skos:definition xml:lang="en">This element indicates a common declaration, a specific part of a document, in
            general in international agreements.
        </skos:definition>
        <skos:inScheme rdf:resource="http://publications.europa.eu/resource/authority/subdivision"/>
        <skos:topConceptOf rdf:resource="http://publications.europa.eu/resource/authority/subdivision"/>
        <dc:identifier>DCL</dc:identifier>
        <atold:op-code>DCL</atold:op-code>
        <at:op-code>DCL</at:op-code>
        <at:start.use>1952-12-30</at:start.use>
        <at:authority-code>DCL</at:authority-code>
        <skos:notation rdf:datatype="http://publications.europa.eu/ontology/euvoc#FORMEX">DC</skos:notation>
        <at:op-mapped-code>
            <at:MappedCode>
                <dc:source>FORMEX</dc:source>
                <at:legacy-code>DC</at:legacy-code>
            </at:MappedCode>
        </at:op-mapped-code>
    </skos:Concept>
    <skos:Concept rdf:about="http://publications.europa.eu/resource/authority/subdivision/ANX"
                  at:deprecated="false">
        <skos:prefLabel xml:lang="sv">bilaga</skos:prefLabel>
        <skos:prefLabel xml:lang="en">annex</skos:prefLabel>
        <skos:definition xml:lang="en">distinct part of an act that generally contains rules or technical data which,
            for practical reasons, do not appear in the enacting terms, and frequently take the form of a list or table
        </skos:definition>
        <skos:inScheme rdf:resource="http://publications.europa.eu/resource/authority/subdivision"/>
        <skos:topConceptOf rdf:resource="http://publications.europa.eu/resource/authority/subdivision"/>
        <dc:identifier>ANX</dc:identifier>
        <atold:op-code>ANX</atold:op-code>
        <at:op-code>ANX</at:op-code>
        <at:start.use>2015-03-18</at:start.use>
        <at:authority-code>ANX</at:authority-code>
        <skos:notation rdf:datatype="http://publications.europa.eu/ontology/euvoc#CJ">N</skos:notation>
        <skos:notation rdf:datatype="http://publications.europa.eu/ontology/euvoc#FORMEX">AX</skos:notation>
        <at:op-mapped-code>
            <at:MappedCode>
                <dc:source>CJ</dc:source>
                <at:legacy-code>N</at:legacy-code>
            </at:MappedCode>
        </at:op-mapped-code>
        <at:op-mapped-code>
            <at:MappedCode>
                <dc:source>FORMEX</dc:source>
                <at:legacy-code>AX</at:legacy-code>
            </at:MappedCode>
        </at:op-mapped-code>
    </skos:Concept>
    <skos:Concept rdf:about="http://publications.europa.eu/resource/authority/subdivision/PBL"
                  at:deprecated="false">
        <skos:prefLabel xml:lang="en">preamble</skos:prefLabel>
        <skos:prefLabel xml:lang="sv">ingress</skos:prefLabel>
        <skos:definition xml:lang="en">part of an act positioned after the title of the act that includes the citations,
            the recitals and the solemn forms preceding the enacting terms
        </skos:definition>
        <skos:inScheme rdf:resource="http://publications.europa.eu/resource/authority/subdivision"/>
        <skos:topConceptOf rdf:resource="http://publications.europa.eu/resource/authority/subdivision"/>
        <dc:identifier>PBL</dc:identifier>
        <atold:op-code>PBL</atold:op-code>
        <at:op-code>PBL</at:op-code>
        <at:start.use>2015-03-18</at:start.use>
        <at:authority-code>PBL</at:authority-code>
        <skos:notation rdf:datatype="http://publications.europa.eu/ontology/euvoc#FORMEX">PB</skos:notation>
        <skos:notation rdf:datatype="http://publications.europa.eu/ontology/euvoc#CJ">PR</skos:notation>
        <at:op-mapped-code>
            <at:MappedCode>
                <dc:source>FORMEX</dc:source>
                <at:legacy-code>PB</at:legacy-code>
            </at:MappedCode>
        </at:op-mapped-code>
        <at:op-mapped-code>
            <at:MappedCode>
                <dc:source>CJ</dc:source>
                <at:legacy-code>PR</at:legacy-code>
            </at:MappedCode>
        </at:op-mapped-code>
    </skos:Concept>
    <skos:Concept rdf:about="http://publications.europa.eu/resource/authority/subdivision/SFR"
                  at:deprecated="false">
        <skos:prefLabel xml:lang="en">scientific formula</skos:prefLabel>
        <skos:prefLabel xml:lang="sv">vetenskaplig formel</skos:prefLabel>
        <skos:definition xml:lang="en">complex technical or scientific expression</skos:definition>
        <skos:inScheme rdf:resource="http://publications.europa.eu/resource/authority/subdivision"/>
        <skos:topConceptOf rdf:resource="http://publications.europa.eu/resource/authority/subdivision"/>
        <dc:identifier>SFR</dc:identifier>
        <atold:op-code>SFR</atold:op-code>
        <at:op-code>SFR</at:op-code>
        <at:start.use>1952-12-30</at:start.use>
        <at:authority-code>SFR</at:authority-code>
    </skos:Concept>
    <skos:Concept rdf:about="http://publications.europa.eu/resource/authority/subdivision/SCT"
                  at:deprecated="false">
        <skos:prefLabel xml:lang="sv">avsnitt</skos:prefLabel>
        <skos:prefLabel xml:lang="en">section</skos:prefLabel>
        <skos:definition xml:lang="en">lowest of the four higher subdivisions of an act (others are parts, titles and
            chapters) used to introduce a group of articles in the enacting terms
        </skos:definition>
        <skos:inScheme rdf:resource="http://publications.europa.eu/resource/authority/subdivision"/>
        <skos:topConceptOf rdf:resource="http://publications.europa.eu/resource/authority/subdivision"/>
        <dc:identifier>SCT</dc:identifier>
        <atold:op-code>SCT</atold:op-code>
        <at:op-code>SCT</at:op-code>
        <at:start.use>2015-03-18</at:start.use>
        <at:authority-code>SCT</at:authority-code>
        <skos:scopeNote xml:lang="en">Sections have distinctive signs of type Arab numerals 1, 2, 3 etc.
        </skos:scopeNote>
        <skos:notation rdf:datatype="http://publications.europa.eu/ontology/euvoc#CJ">S</skos:notation>
        <skos:notation rdf:datatype="http://publications.europa.eu/ontology/euvoc#FORMEX">SE</skos:notation>
        <at:op-mapped-code>
            <at:MappedCode>
                <dc:source>CJ</dc:source>
                <at:legacy-code>S</at:legacy-code>
            </at:MappedCode>
        </at:op-mapped-code>
        <at:op-mapped-code>
            <at:MappedCode>
                <dc:source>FORMEX</dc:source>
                <at:legacy-code>SE</at:legacy-code>
            </at:MappedCode>
        </at:op-mapped-code>
    </skos:Concept>
    <skos:Concept rdf:about="http://publications.europa.eu/resource/authority/subdivision/FGR"
                  at:deprecated="false">
        <skos:prefLabel xml:lang="sv">figur</skos:prefLabel>
        <skos:prefLabel xml:lang="en">figure</skos:prefLabel>
        <skos:definition xml:lang="en">image supplemented by related text</skos:definition>
        <skos:altLabel xml:lang="en">image</skos:altLabel>
        <skos:inScheme rdf:resource="http://publications.europa.eu/resource/authority/subdivision"/>
        <skos:topConceptOf rdf:resource="http://publications.europa.eu/resource/authority/subdivision"/>
        <dc:identifier>FGR</dc:identifier>
        <atold:op-code>FGR</atold:op-code>
        <at:op-code>FGR</at:op-code>
        <at:start.use>1952-12-30</at:start.use>
        <at:authority-code>FGR</at:authority-code>
        <skos:notation rdf:datatype="http://publications.europa.eu/ontology/euvoc#FORMEX">FG</skos:notation>
        <at:op-mapped-code>
            <at:MappedCode>
                <dc:source>FORMEX</dc:source>
                <at:legacy-code>FG</at:legacy-code>
            </at:MappedCode>
        </at:op-mapped-code>
    </skos:Concept>
    <skos:Concept rdf:about="http://publications.europa.eu/resource/authority/subdivision/LST"
                  at:deprecated="false">
        <skos:prefLabel xml:lang="en">list</skos:prefLabel>
        <skos:prefLabel xml:lang="sv">förteckning</skos:prefLabel>
        <skos:definition xml:lang="en">This element indicates information structured by means of a list in a legal
            document.
        </skos:definition>
        <skos:inScheme rdf:resource="http://publications.europa.eu/resource/authority/subdivision"/>
        <skos:topConceptOf rdf:resource="http://publications.europa.eu/resource/authority/subdivision"/>
        <dc:identifier>LST</dc:identifier>
        <atold:op-code>LST</atold:op-code>
        <at:op-code>LST</at:op-code>
        <at:start.use>1952-12-30</at:start.use>
        <at:authority-code>LST</at:authority-code>
        <skos:notation rdf:datatype="http://publications.europa.eu/ontology/euvoc#FORMEX">LI</skos:notation>
        <at:op-mapped-code>
            <at:MappedCode>
                <dc:source>FORMEX</dc:source>
                <at:legacy-code>LI</at:legacy-code>
            </at:MappedCode>
        </at:op-mapped-code>
    </skos:Concept>
    <skos:Concept rdf:about="http://publications.europa.eu/resource/authority/subdivision/SUB"
                  at:deprecated="false">
        <skos:prefLabel xml:lang="sv">stycke</skos:prefLabel>
        <skos:prefLabel xml:lang="en">subparagraph</skos:prefLabel>
        <skos:definition xml:lang="en">first level of an unnumbered subdivision of a numbered paragraph, point or
            indent, where there are at least two of such elements of subdivision
        </skos:definition>
        <skos:inScheme rdf:resource="http://publications.europa.eu/resource/authority/subdivision"/>
        <skos:topConceptOf rdf:resource="http://publications.europa.eu/resource/authority/subdivision"/>
        <dc:identifier>SUB</dc:identifier>
        <atold:op-code>SUB</atold:op-code>
        <at:op-code>SUB</at:op-code>
        <at:start.use>1952-12-30</at:start.use>
        <at:authority-code>SUB</at:authority-code>
    </skos:Concept>
    <skos:Concept rdf:about="http://publications.europa.eu/resource/authority/subdivision/SNT"
                  at:deprecated="false">
        <skos:prefLabel xml:lang="sv">mening</skos:prefLabel>
        <skos:prefLabel xml:lang="en">sentence</skos:prefLabel>
        <skos:definition xml:lang="en">A sentence is a linguistic unit of grammatically linked words. This subdivision
            can be cited.
        </skos:definition>
        <skos:inScheme rdf:resource="http://publications.europa.eu/resource/authority/subdivision"/>
        <skos:topConceptOf rdf:resource="http://publications.europa.eu/resource/authority/subdivision"/>
        <dc:identifier>SNT</dc:identifier>
        <atold:op-code>SNT</atold:op-code>
        <at:op-code>SNT</at:op-code>
        <at:start.use>1952-12-30</at:start.use>
        <at:authority-code>SNT</at:authority-code>
    </skos:Concept>
    <skos:Concept rdf:about="http://publications.europa.eu/resource/authority/subdivision/RCT"
                  at:deprecated="false">
        <skos:prefLabel xml:lang="sv">skäl</skos:prefLabel>
        <skos:prefLabel xml:lang="en">recital</skos:prefLabel>
        <skos:definition xml:lang="en">element in the preamble that sets out the reasoning for the chief provisions of
            the enacting terms
        </skos:definition>
        <skos:inScheme rdf:resource="http://publications.europa.eu/resource/authority/subdivision"/>
        <skos:topConceptOf rdf:resource="http://publications.europa.eu/resource/authority/subdivision"/>
        <dc:identifier>RCT</dc:identifier>
        <atold:op-code>RCT</atold:op-code>
        <at:op-code>RCT</at:op-code>
        <at:start.use>2015-03-18</at:start.use>
        <at:authority-code>RCT</at:authority-code>
        <skos:notation rdf:datatype="http://publications.europa.eu/ontology/euvoc#FORMEX">CO</skos:notation>
        <skos:notation rdf:datatype="http://publications.europa.eu/ontology/euvoc#CJ">C</skos:notation>
        <at:op-mapped-code>
            <at:MappedCode>
                <dc:source>CJ</dc:source>
                <at:legacy-code>C</at:legacy-code>
            </at:MappedCode>
        </at:op-mapped-code>
        <at:op-mapped-code>
            <at:MappedCode>
                <dc:source>FORMEX</dc:source>
                <at:legacy-code>CO</at:legacy-code>
            </at:MappedCode>
        </at:op-mapped-code>
    </skos:Concept>
    <skos:Concept rdf:about="http://publications.europa.eu/resource/authority/subdivision/TAB"
                  at:deprecated="false">
        <skos:prefLabel xml:lang="en">table</skos:prefLabel>
        <skos:prefLabel xml:lang="sv">tabell</skos:prefLabel>
        <skos:definition xml:lang="en">This element indicates a table in a legal document containing text structured in
            rows and columns with the related data.
        </skos:definition>
        <skos:inScheme rdf:resource="http://publications.europa.eu/resource/authority/subdivision"/>
        <skos:topConceptOf rdf:resource="http://publications.europa.eu/resource/authority/subdivision"/>
        <dc:identifier>TAB</dc:identifier>
        <atold:op-code>TAB</atold:op-code>
        <at:op-code>TAB</at:op-code>
        <at:start.use>1952-12-30</at:start.use>
        <at:authority-code>TAB</at:authority-code>
        <skos:notation rdf:datatype="http://publications.europa.eu/ontology/euvoc#FORMEX">TA</skos:notation>
        <at:op-mapped-code>
            <at:MappedCode>
                <dc:source>FORMEX</dc:source>
                <at:legacy-code>TA</at:legacy-code>
            </at:MappedCode>
        </at:op-mapped-code>
    </skos:Concept>
    <skos:Concept rdf:about="http://publications.europa.eu/resource/authority/subdivision/ROW"
                  at:deprecated="false">
        <skos:prefLabel xml:lang="en">table row</skos:prefLabel>
        <skos:prefLabel xml:lang="sv">tabellrad</skos:prefLabel>
        <skos:definition xml:lang="en">horizontal arrangement of data in a table</skos:definition>
        <skos:inScheme rdf:resource="http://publications.europa.eu/resource/authority/subdivision"/>
        <skos:topConceptOf rdf:resource="http://publications.europa.eu/resource/authority/subdivision"/>
        <dc:identifier>ROW</dc:identifier>
        <atold:op-code>ROW</atold:op-code>
        <at:op-code>ROW</at:op-code>
        <at:start.use>1952-12-30</at:start.use>
        <at:authority-code>ROW</at:authority-code>
        <skos:notation rdf:datatype="http://publications.europa.eu/ontology/euvoc#FORMEX">RO</skos:notation>
        <at:op-mapped-code>
            <at:MappedCode>
                <dc:source>FORMEX</dc:source>
                <at:legacy-code>RO</at:legacy-code>
            </at:MappedCode>
        </at:op-mapped-code>
    </skos:Concept>
    <skos:Concept rdf:about="http://publications.europa.eu/resource/authority/subdivision/INP"
                  at:deprecated="false">
        <skos:prefLabel xml:lang="en">introductory part</skos:prefLabel>
        <skos:prefLabel xml:lang="sv">inledande del</skos:prefLabel>
        <skos:definition xml:lang="en">one or more sentences or phrases in the beginning of a paragraph, or of a
            subparagraph, or of a point, preceding an enumeration (of points or indents) and ending with a colon ‘:’
        </skos:definition>
        <skos:inScheme rdf:resource="http://publications.europa.eu/resource/authority/subdivision"/>
        <skos:topConceptOf rdf:resource="http://publications.europa.eu/resource/authority/subdivision"/>
        <dc:identifier>INP</dc:identifier>
        <atold:op-code>INP</atold:op-code>
        <at:op-code>INP</at:op-code>
        <at:start.use>1952-12-30</at:start.use>
        <at:authority-code>INP</at:authority-code>
    </skos:Concept>
    <skos:Concept rdf:about="http://publications.europa.eu/resource/authority/subdivision/CGR"
                  at:deprecated="false">
        <skos:prefLabel xml:lang="en">group of corrections</skos:prefLabel>
        <skos:prefLabel xml:lang="sv">grupp av rättelser</skos:prefLabel>
        <skos:definition xml:lang="en">This element is specific to the corrigendum type of document. It is used to mark
            up two or more corrections that have a common introductory sentence.
        </skos:definition>
        <skos:inScheme rdf:resource="http://publications.europa.eu/resource/authority/subdivision"/>
        <skos:topConceptOf rdf:resource="http://publications.europa.eu/resource/authority/subdivision"/>
        <dc:identifier>CGR</dc:identifier>
        <atold:op-code>CGR</atold:op-code>
        <at:op-code>CGR</at:op-code>
        <at:start.use>2004-05-01</at:start.use>
        <at:authority-code>CGR</at:authority-code>
    </skos:Concept>
    <skos:Concept rdf:about="http://publications.europa.eu/resource/authority/subdivision/IMG"
                  at:deprecated="false">
        <skos:prefLabel xml:lang="en">image</skos:prefLabel>
        <skos:prefLabel xml:lang="sv">bild</skos:prefLabel>
        <skos:definition xml:lang="en">graphical element depicting an object which may contain alphanumeric data
        </skos:definition>
        <skos:inScheme rdf:resource="http://publications.europa.eu/resource/authority/subdivision"/>
        <skos:topConceptOf rdf:resource="http://publications.europa.eu/resource/authority/subdivision"/>
        <dc:identifier>IMG</dc:identifier>
        <atold:op-code>IMG</atold:op-code>
        <at:op-code>IMG</at:op-code>
        <at:start.use>1952-12-30</at:start.use>
        <at:authority-code>IMG</at:authority-code>
    </skos:Concept>
    <skos:Concept rdf:about="http://publications.europa.eu/resource/authority/subdivision/PNT"
                  at:deprecated="false">
        <skos:prefLabel xml:lang="en">point</skos:prefLabel>
        <skos:prefLabel xml:lang="sv">led</skos:prefLabel>
        <skos:definition xml:lang="en">structure component of a legal article that has a distinctive sign of the type
            Arabic numbers: (1), (2), (3) etc.
        </skos:definition>
        <skos:inScheme rdf:resource="http://publications.europa.eu/resource/authority/subdivision"/>
        <skos:topConceptOf rdf:resource="http://publications.europa.eu/resource/authority/subdivision"/>
        <dc:identifier>PNT</dc:identifier>
        <atold:op-code>PNT</atold:op-code>
        <at:op-code>PNT</at:op-code>
        <at:start.use>2015-03-18</at:start.use>
        <at:authority-code>PNT</at:authority-code>
        <skos:scopeNote xml:lang="en">Indicates either each element of an enumeration inside a paragraph, a subparagraph
            or a point (this enumeration being generally preceded by an introductory phrase); or is possibly used
            independently as a basic unit, e.g. in annexes or preparatory documents.
        </skos:scopeNote>
        <skos:notation rdf:datatype="http://publications.europa.eu/ontology/euvoc#CJ">PT</skos:notation>
        <skos:notation rdf:datatype="http://publications.europa.eu/ontology/euvoc#FORMEX">PT</skos:notation>
        <at:op-mapped-code>
            <at:MappedCode>
                <dc:source>CJ</dc:source>
                <at:legacy-code>PT</at:legacy-code>
            </at:MappedCode>
        </at:op-mapped-code>
        <at:op-mapped-code>
            <at:MappedCode>
                <dc:source>FORMEX</dc:source>
                <at:legacy-code>PT</at:legacy-code>
            </at:MappedCode>
        </at:op-mapped-code>
    </skos:Concept>
    <skos:Concept rdf:about="http://publications.europa.eu/resource/authority/subdivision/AGR"
                  at:deprecated="false">
        <skos:prefLabel xml:lang="en">agreement</skos:prefLabel>
        <skos:prefLabel xml:lang="sv">avtal</skos:prefLabel>
        <skos:definition xml:lang="en">This element indicates an agreement as part of an act.</skos:definition>
        <skos:inScheme rdf:resource="http://publications.europa.eu/resource/authority/subdivision"/>
        <skos:topConceptOf rdf:resource="http://publications.europa.eu/resource/authority/subdivision"/>
        <dc:identifier>AGR</dc:identifier>
        <atold:op-code>AGR</atold:op-code>
        <at:op-code>AGR</at:op-code>
        <at:start.use>1952-07-24</at:start.use>
        <at:authority-code>AGR</at:authority-code>
    </skos:Concept>
    <skos:Concept rdf:about="http://publications.europa.eu/resource/authority/subdivision/FNP"
                  at:deprecated="false">
        <skos:prefLabel xml:lang="en">final part</skos:prefLabel>
        <skos:prefLabel xml:lang="sv">avslutande del</skos:prefLabel>
        <skos:definition xml:lang="en">This element indicates the final part of a legal act which follows the enacting
            terms. The final part contains the place, date and signatures and sometimes also the rule of application.
        </skos:definition>
        <skos:inScheme rdf:resource="http://publications.europa.eu/resource/authority/subdivision"/>
        <skos:topConceptOf rdf:resource="http://publications.europa.eu/resource/authority/subdivision"/>
        <dc:identifier>FNP</dc:identifier>
        <atold:op-code>FNP</atold:op-code>
        <at:op-code>FNP</at:op-code>
        <at:start.use>1952-12-30</at:start.use>
        <at:authority-code>FNP</at:authority-code>
        <skos:notation rdf:datatype="http://publications.europa.eu/ontology/euvoc#FORMEX">FI</skos:notation>
        <at:op-mapped-code>
            <at:MappedCode>
                <dc:source>FORMEX</dc:source>
                <at:legacy-code>FI</at:legacy-code>
            </at:MappedCode>
        </at:op-mapped-code>
    </skos:Concept>
    <skos:Concept rdf:about="http://publications.europa.eu/resource/authority/subdivision/PRO"
                  at:deprecated="false">
        <skos:prefLabel xml:lang="sv">protokoll</skos:prefLabel>
        <skos:prefLabel xml:lang="en">protocol</skos:prefLabel>
        <skos:definition xml:lang="en">This element indicates a protocol, a specific part of a legal document.
        </skos:definition>
        <skos:inScheme rdf:resource="http://publications.europa.eu/resource/authority/subdivision"/>
        <skos:topConceptOf rdf:resource="http://publications.europa.eu/resource/authority/subdivision"/>
        <dc:identifier>PRO</dc:identifier>
        <atold:op-code>PRO</atold:op-code>
        <at:op-code>PRO</at:op-code>
        <at:start.use>1952-12-30</at:start.use>
        <at:authority-code>PRO</at:authority-code>
        <skos:notation rdf:datatype="http://publications.europa.eu/ontology/euvoc#FORMEX">PC</skos:notation>
        <at:op-mapped-code>
            <at:MappedCode>
                <dc:source>FORMEX</dc:source>
                <at:legacy-code>PC</at:legacy-code>
            </at:MappedCode>
        </at:op-mapped-code>
    </skos:Concept>
    <skos:Concept rdf:about="http://publications.europa.eu/resource/authority/subdivision/MNT"
                  at:deprecated="false">
        <skos:prefLabel xml:lang="sv">protokoll</skos:prefLabel>
        <skos:prefLabel xml:lang="en">minutes</skos:prefLabel>
        <skos:definition xml:lang="en">This element indicates minutes, a specific part of a document, e.g. in a
            treaty.
        </skos:definition>
        <skos:inScheme rdf:resource="http://publications.europa.eu/resource/authority/subdivision"/>
        <skos:topConceptOf rdf:resource="http://publications.europa.eu/resource/authority/subdivision"/>
        <dc:identifier>MNT</dc:identifier>
        <atold:op-code>MNT</atold:op-code>
        <at:op-code>MNT</at:op-code>
        <at:start.use>1952-12-30</at:start.use>
        <at:authority-code>MNT</at:authority-code>
    </skos:Concept>
    <skos:Concept rdf:about="http://publications.europa.eu/resource/authority/subdivision/CNV"
                  at:deprecated="false">
        <skos:prefLabel xml:lang="en">convention</skos:prefLabel>
        <skos:prefLabel xml:lang="sv">konvention</skos:prefLabel>
        <skos:definition xml:lang="en">This element indicates a convention, a specific part of a document, e.g. in a
            treaty.
        </skos:definition>
        <skos:inScheme rdf:resource="http://publications.europa.eu/resource/authority/subdivision"/>
        <skos:topConceptOf rdf:resource="http://publications.europa.eu/resource/authority/subdivision"/>
        <dc:identifier>CNV</dc:identifier>
        <atold:op-code>CNV</atold:op-code>
        <at:op-code>CNV</at:op-code>
        <at:start.use>1952-12-30</at:start.use>
        <at:authority-code>CNV</at:authority-code>
    </skos:Concept>
    <skos:Concept rdf:about="http://publications.europa.eu/resource/authority/subdivision/TIT"
                  at:deprecated="false">
        <skos:prefLabel xml:lang="sv">titel</skos:prefLabel>
        <skos:prefLabel xml:lang="en">title</skos:prefLabel>
        <skos:definition xml:lang="en">designation of an act or the designation of a subdivision (e.g. article, chapter,
            part) of an act
        </skos:definition>
        <skos:inScheme rdf:resource="http://publications.europa.eu/resource/authority/subdivision"/>
        <skos:topConceptOf rdf:resource="http://publications.europa.eu/resource/authority/subdivision"/>
        <dc:identifier>TIT</dc:identifier>
        <atold:op-code>TIT</atold:op-code>
        <at:op-code>TIT</at:op-code>
        <at:start.use>2015-03-18</at:start.use>
        <at:authority-code>TIT</at:authority-code>
        <skos:scopeNote xml:lang="en">The Common Vocabulary (CoV) definition ‘The title of the document comprises all
            the information in the heading of the document which serves to identify it’ is referring to the same.
        </skos:scopeNote>
        <skos:scopeNote xml:lang="en">The complete title of an act comprises type of act, number of act, name of the
            author of the act, date of adoption and subject matter. In the case of subdivisions, the title contains the
            subject matter.
        </skos:scopeNote>
        <skos:notation rdf:datatype="http://publications.europa.eu/ontology/euvoc#FORMEX">TI</skos:notation>
        <skos:notation rdf:datatype="http://publications.europa.eu/ontology/euvoc#CJ">TIT</skos:notation>
        <at:op-mapped-code>
            <at:MappedCode>
                <dc:source>CJ</dc:source>
                <at:legacy-code>TIT</at:legacy-code>
            </at:MappedCode>
        </at:op-mapped-code>
        <at:op-mapped-code>
            <at:MappedCode>
                <dc:source>FORMEX</dc:source>
                <at:legacy-code>TI</at:legacy-code>
            </at:MappedCode>
        </at:op-mapped-code>
    </skos:Concept>
    <skos:Concept rdf:about="http://publications.europa.eu/resource/authority/subdivision/LGD"
                  at:deprecated="false">
        <skos:prefLabel xml:lang="sv">förklaring</skos:prefLabel>
        <skos:prefLabel xml:lang="en">legend</skos:prefLabel>
        <skos:definition xml:lang="en">text detailing the meaning of the elements of an image, a table or a scientific
            formula it relates to
        </skos:definition>
        <skos:inScheme rdf:resource="http://publications.europa.eu/resource/authority/subdivision"/>
        <skos:topConceptOf rdf:resource="http://publications.europa.eu/resource/authority/subdivision"/>
        <dc:identifier>LGD</dc:identifier>
        <atold:op-code>LGD</atold:op-code>
        <at:op-code>LGD</at:op-code>
        <at:start.use>1952-12-30</at:start.use>
        <at:authority-code>LGD</at:authority-code>
    </skos:Concept>
    <skos:Concept rdf:about="http://publications.europa.eu/resource/authority/subdivision/RUL"
                  at:deprecated="false">
        <skos:prefLabel xml:lang="sv">regel</skos:prefLabel>
        <skos:prefLabel xml:lang="en">rule</skos:prefLabel>
        <skos:definition xml:lang="en">The RULE element is used in some acts, such as in Commission Regulation (EC) No
            2868/95 of 13 December 1995.
        </skos:definition>
        <skos:inScheme rdf:resource="http://publications.europa.eu/resource/authority/subdivision"/>
        <skos:topConceptOf rdf:resource="http://publications.europa.eu/resource/authority/subdivision"/>
        <dc:identifier>RUL</dc:identifier>
        <atold:op-code>RUL</atold:op-code>
        <at:op-code>RUL</at:op-code>
        <at:start.use>2015-03-18</at:start.use>
        <at:authority-code>RUL</at:authority-code>
        <skos:notation rdf:datatype="http://publications.europa.eu/ontology/euvoc#CJ">R</skos:notation>
        <at:op-mapped-code>
            <at:MappedCode>
                <dc:source>CJ</dc:source>
                <at:legacy-code>R</at:legacy-code>
            </at:MappedCode>
        </at:op-mapped-code>
    </skos:Concept>
    <skos:Concept rdf:about="http://publications.europa.eu/resource/authority/subdivision/PAG"
                  at:deprecated="false">
        <skos:prefLabel xml:lang="sv">sida</skos:prefLabel>
        <skos:prefLabel xml:lang="en">page</skos:prefLabel>
        <skos:definition xml:lang="en">This element indicates a subdivision of the basic act of a consolidation,
            specified by page number as given in the original publication in the Official Journal (OJ). The figure added
            to the subdivision indicates the page number in the original publication of the basic act in the OJ.Example:
            PG:40 indicates a position on page 40 in the original publication of the basic act in the OJ.
        </skos:definition>
        <skos:inScheme rdf:resource="http://publications.europa.eu/resource/authority/subdivision"/>
        <skos:topConceptOf rdf:resource="http://publications.europa.eu/resource/authority/subdivision"/>
        <dc:identifier>PAG</dc:identifier>
        <atold:op-code>PAG</atold:op-code>
        <at:op-code>PAG</at:op-code>
        <at:start.use>1952-12-30</at:start.use>
        <at:authority-code>PAG</at:authority-code>
        <skos:notation rdf:datatype="http://publications.europa.eu/ontology/euvoc#FORMEX">PG</skos:notation>
        <at:op-mapped-code>
            <at:MappedCode>
                <dc:source>FORMEX</dc:source>
                <at:legacy-code>PG</at:legacy-code>
            </at:MappedCode>
        </at:op-mapped-code>
    </skos:Concept>
    <skos:Concept rdf:about="http://publications.europa.eu/resource/authority/subdivision/PRT"
                  at:deprecated="false">
        <skos:prefLabel xml:lang="en">part</skos:prefLabel>
        <skos:prefLabel xml:lang="sv">del</skos:prefLabel>
        <skos:definition xml:lang="en">subdivision of a legal document used to introduce a group of articles in the
            enacting terms
        </skos:definition>
        <skos:inScheme rdf:resource="http://publications.europa.eu/resource/authority/subdivision"/>
        <skos:topConceptOf rdf:resource="http://publications.europa.eu/resource/authority/subdivision"/>
        <dc:identifier>PRT</dc:identifier>
        <atold:op-code>PRT</atold:op-code>
        <at:op-code>PRT</at:op-code>
        <at:start.use>2015-03-18</at:start.use>
        <at:authority-code>PRT</at:authority-code>
        <skos:scopeNote xml:lang="en">In the hierarchy of subdivisions, part is above title.</skos:scopeNote>
        <skos:scopeNote xml:lang="en">Parts have distinctive signs of type uppercase Roman numbers I, II, III etc. or
            numbers written by letters, Part One, Part Two, Part Three etc. which can also be referenced as first part,
            second part, third part etc.
        </skos:scopeNote>
        <skos:notation rdf:datatype="http://publications.europa.eu/ontology/euvoc#CJ">PART</skos:notation>
        <skos:notation rdf:datatype="http://publications.europa.eu/ontology/euvoc#FORMEX">PR</skos:notation>
        <at:op-mapped-code>
            <at:MappedCode>
                <dc:source>FORMEX</dc:source>
                <at:legacy-code>PR</at:legacy-code>
            </at:MappedCode>
        </at:op-mapped-code>
        <at:op-mapped-code>
            <at:MappedCode>
                <dc:source>CJ</dc:source>
                <at:legacy-code>PART</at:legacy-code>
            </at:MappedCode>
        </at:op-mapped-code>
    </skos:Concept>
    <skos:Concept rdf:about="http://publications.europa.eu/resource/authority/subdivision/TXO"
                  at:deprecated="false">
        <skos:prefLabel xml:lang="sv">gammal text</skos:prefLabel>
        <skos:prefLabel xml:lang="en">old text</skos:prefLabel>
        <skos:definition xml:lang="en">This element is specific to the corrigendum type of document. It is a subdivision
            of the correction and is used to mark up the original text that was published in a document and should be
            modified by the corrigendum.
        </skos:definition>
        <skos:inScheme rdf:resource="http://publications.europa.eu/resource/authority/subdivision"/>
        <skos:topConceptOf rdf:resource="http://publications.europa.eu/resource/authority/subdivision"/>
        <dc:identifier>TXO</dc:identifier>
        <atold:op-code>TXO</atold:op-code>
        <at:op-code>TXO</at:op-code>
        <at:start.use>2004-05-01</at:start.use>
        <at:authority-code>TXO</at:authority-code>
    </skos:Concept>
    <skos:Concept rdf:about="http://publications.europa.eu/resource/authority/subdivision/END"
                  at:deprecated="false">
        <skos:prefLabel xml:lang="en">endnote</skos:prefLabel>
        <skos:prefLabel xml:lang="sv">slutnot</skos:prefLabel>
        <skos:definition xml:lang="en">reference included in a legal document which is specified in the end of a
            subdivision of an act
        </skos:definition>
        <skos:inScheme rdf:resource="http://publications.europa.eu/resource/authority/subdivision"/>
        <skos:topConceptOf rdf:resource="http://publications.europa.eu/resource/authority/subdivision"/>
        <dc:identifier>END</dc:identifier>
        <atold:op-code>END</atold:op-code>
        <at:op-code>END</at:op-code>
        <at:start.use>1952-12-30</at:start.use>
        <at:authority-code>END</at:authority-code>
        <skos:example xml:lang="en">Commission Regulation (EU) 2015/1005 of 25 June 2015</skos:example>
    </skos:Concept>
    <skos:Concept rdf:about="http://publications.europa.eu/resource/authority/subdivision/PTI"
                  at:deprecated="false">
        <skos:prefLabel xml:lang="en">point</skos:prefLabel>
        <skos:prefLabel xml:lang="sv">led</skos:prefLabel>
        <skos:definition xml:lang="en">structure component of a legal article that has a distinctive sign of the type
            lowercase Roman numbers: (i), (ii), (iii) etc.
        </skos:definition>
        <skos:inScheme rdf:resource="http://publications.europa.eu/resource/authority/subdivision"/>
        <skos:topConceptOf rdf:resource="http://publications.europa.eu/resource/authority/subdivision"/>
        <dc:identifier>PTI</dc:identifier>
        <atold:op-code>PTI</atold:op-code>
        <at:op-code>PTI</at:op-code>
        <at:start.use>1952-12-30</at:start.use>
        <at:authority-code>PTI</at:authority-code>
    </skos:Concept>
    <skos:Concept rdf:about="http://publications.europa.eu/resource/authority/subdivision/PAR"
                  at:deprecated="false">
        <skos:prefLabel xml:lang="sv">punkt</skos:prefLabel>
        <skos:prefLabel xml:lang="en">paragraph</skos:prefLabel>
        <skos:definition xml:lang="en">The PAR element is used to mark up a subdivision of an article numbered using
            Arab numerals within a European legal text. It is made up of at least one alinea or quoted text.
        </skos:definition>
        <skos:altLabel xml:lang="en">numbered paragraph</skos:altLabel>
        <skos:inScheme rdf:resource="http://publications.europa.eu/resource/authority/subdivision"/>
        <skos:topConceptOf rdf:resource="http://publications.europa.eu/resource/authority/subdivision"/>
        <dc:identifier>PAR</dc:identifier>
        <atold:op-code>PAR</atold:op-code>
        <at:op-code>PAR</at:op-code>
        <at:start.use>2015-03-18</at:start.use>
        <at:authority-code>PAR</at:authority-code>
        <skos:notation rdf:datatype="http://publications.europa.eu/ontology/euvoc#CJ">P</skos:notation>
        <skos:notation rdf:datatype="http://publications.europa.eu/ontology/euvoc#FORMEX">PA</skos:notation>
        <at:op-mapped-code>
            <at:MappedCode>
                <dc:source>CJ</dc:source>
                <at:legacy-code>P</at:legacy-code>
            </at:MappedCode>
        </at:op-mapped-code>
        <at:op-mapped-code>
            <at:MappedCode>
                <dc:source>FORMEX</dc:source>
                <at:legacy-code>PA</at:legacy-code>
            </at:MappedCode>
        </at:op-mapped-code>
    </skos:Concept>
    <skos:Concept rdf:about="http://publications.europa.eu/resource/authority/subdivision/OP_DATPRO"
                  at:deprecated="false">
        <skos:prefLabel xml:lang="en">Provisional data</skos:prefLabel>
        <skos:prefLabel xml:lang="sv">Tillfälliga uppgifter</skos:prefLabel>
        <skos:inScheme rdf:resource="http://publications.europa.eu/resource/authority/subdivision"/>
        <skos:topConceptOf rdf:resource="http://publications.europa.eu/resource/authority/subdivision"/>
        <dc:identifier>OP_DATPRO</dc:identifier>
        <atold:op-code>OP_DATPRO</atold:op-code>
        <at:op-code>OP_DATPRO</at:op-code>
        <at:start.use>1952-07-23</at:start.use>
        <at:authority-code>OP_DATPRO</at:authority-code>
    </skos:Concept>
</rdf:RDF>
